tapl/tapl.lean
@@ -1,3 +1,4 @@
 import tapl.s03untyped
 import tapl.s05lambdaCalculus
 import tapl.s06nameless
+import tapl.s09types
